Prove subtype_to_vl_subtype pretending we have substitution
- Turn vl_to_tm into an axiom that turns terms into closed values (which we
  can't, but we assume we can with substitution).
- Use it for the intended proof of subtype_to_vl_subtype.

ecoop17/dot_wfrel2.v
@@ -450,15 +450,23 @@ Proof.
   intros; vtp_simpl_unfold; repeat case_match; ev; intros; try injections_some; try contradiction; eauto.
 Qed.
 
-Program Definition vl_to_tm (v : vl): { (e, env) : tm * venv | forall n, forall Hfuel : n > 0, tevalS e n env = Some (Some v, 0) } :=
-  match v with
-  | vabs env T body =>
-    (tabs T body, env)
-  | vty env T =>
-    (ttyp T, env)
-  end.
-Solve Obligations with program_simplify; destruct n; solve [inverse Hfuel] || reflexivity.
+(* Program Definition vl_to_tm (v : vl): { (e, env) : tm * venv | *)
+(*                                         tevalSnmOpt env e (Some v) 0 0 } := *)
+(*   match v with *)
+(*   | vabs env T body => *)
+(*     (tabs T body, env) *)
+(*   | vty env T => *)
+(*     (ttyp T, env) *)
+(*   end. *)
+(* Solve Obligations with program_simplify; unfold tevalSnmOpt in *; intros * Hfuel; destruct n; solve [inverse Hfuel] || reflexivity. *)
 
+(* XXX this isn't true, but we should be able to fix it in a setting with substitution in terms (which depends on substitution in types). *)
+(* Once we define the OFE of semantic types, we can alternatively define a
+language of term realizers that mention no types, not even in ttyp, just like in
+Ahmed's typeless System F. *)
+(* Instead of writing [], just write arbitrary environments right away. *)
+Axiom vl_to_tm: forall (v : vl) , { e : tm | forall env,
+                                 tevalSnmOpt env e (Some v) 0 0 }.
 
 (* We want to relate etp and vtp. *)
 Lemma etp_vtp_j: forall e v k j nm T env,
@@ -506,27 +514,25 @@ Hint Resolve vtp_etp.
 Lemma subtype_to_vl_subtype : forall G T1 T2,
     sem_subtype G T1 T2 -> sem_vl_subtype G T1 T2.
 Proof.
-  unfold sem_subtype, sem_vl_subtype; intros * (? & ? & H).
-  split_conj; eauto.
-  intros * Henv * HvT1.
-  destruct (vl_to_tm v) as [[e env1] Heval]; eauto.
-  (* Here we can't go on because Heval references env1, not env. *)
-  specialize (H k env Henv e).
-  assert (etp T2 k e env) as [? HeT2]. {
-    apply H.
-    unfold etp, expr_sem. split_conj; eauto; intros.
-    unfold etp, expr_sem, tevalSnOpt, tevalSnOpt, tevalSnmOpt in *.
-    ev.
-    exists v.
-    admit.
-  }
-  unfold etp, expr_sem, tevalSnOpt, tevalSnOpt, tevalSnmOpt in HeT2.
-  destruct (HeT2 (Some v) 0) as (? & ? & ?); replace (k - 0) with k in * by omega; simpl; eauto.
-  admit.
-  (* Either: *)
-  congruence.
-  (* injections_some; auto. *)
-Admitted.
+  (* unfold sem_subtype, sem_vl_subtype; intros; intuition eauto; *)
+  (*   destruct (vl_to_tm v) as [e Heval]; firstorder eauto. *)
+  unfold sem_subtype, sem_vl_subtype; intros * (? & ? & Hsub);
+    split_conj; eauto;
+      intros * Henv * HvT1;
+      destruct (vl_to_tm v) as [e Heval];
+      firstorder eauto.
+  (* specialize (Hsub k env Henv e); *)
+  (*   specialize (Heval env). *)
+  (*   (* assert (wf G T1) by eauto. *) *)
+  (* assert (etp T2 k e env) as [? HeT2]. { *)
+  (*   unfold etp, expr_sem in *; apply Hsub; intuition eauto. *)
+  (*   exists v; unfold tevalSnOpt in *; ev; eval_det; eauto. *)
+  (* } *)
+  (* (* eauto. *) *)
+  (* (* (* unfold etp, expr_sem, tevalSnOpt, tevalSnOpt, tevalSnmOpt in HeT2. *) *) *)
+  (* (* (* eauto. *) *) *)
+  (* (* (* destruct (HeT2 (Some v) 0) as (? & ? & ?); replace (k - 0) with k in * by omega; simpl. eauto. *) *) *)
+Qed.
 
 (* Qed. *)
 Hint Resolve subtype_to_vl_subtype.
